<?xml version="1.0"?>


<!DOCTYPE rdf:RDF [
    <!ENTITY dcterms "http://purl.org/dc/terms/" >
    <!ENTITY foaf "http://xmlns.com/foaf/0.1/" >
    <!ENTITY vann "http://purl.org/vocab/vann/" >
    <!ENTITY ns "http://creativecommons.org/ns#" >
    <!ENTITY owl "http://www.w3.org/2002/07/owl#" >
    <!ENTITY dc "http://purl.org/dc/elements/1.1/" >
    <!ENTITY xsd "http://www.w3.org/2001/XMLSchema#" >
    <!ENTITY skos "http://www.w3.org/2004/02/skos/core#" >
    <!ENTITY rdfs "http://www.w3.org/2000/01/rdf-schema#" >
    <!ENTITY wgs84_pos "http://www.w3.org/2003/01/geo/wgs84_pos#" >
    <!ENTITY rdf "http://www.w3.org/1999/02/22-rdf-syntax-ns#" >
    <!ENTITY noise "http://vocab.linkeddata.es/datosabiertos/def/medio-ambiente/contaminacion-acustica#" >
]>


<rdf:RDF xmlns="http://vocab.linkeddata.es/datosabiertos/def/medio-ambiente/contaminacion-acustica#"
     xml:base="http://vocab.linkeddata.es/datosabiertos/def/medio-ambiente/contaminacion-acustica"
     xmlns:dc="http://purl.org/dc/elements/1.1/"
     xmlns:ns="http://creativecommons.org/ns#"
     xmlns:wgs84_pos="http://www.w3.org/2003/01/geo/wgs84_pos#"
     xmlns:foaf="http://xmlns.com/foaf/0.1/"
     xmlns:vann="http://purl.org/vocab/vann/"
     xmlns:dcterms="http://purl.org/dc/terms/"
     xmlns:noise="http://vocab.linkeddata.es/datosabiertos/def/medio-ambiente/contaminacion-acustica#"
     xmlns:rdfs="http://www.w3.org/2000/01/rdf-schema#"
     xmlns:owl="http://www.w3.org/2002/07/owl#"
     xmlns:xsd="http://www.w3.org/2001/XMLSchema#"
     xmlns:rdf="http://www.w3.org/1999/02/22-rdf-syntax-ns#"
     xmlns:skos="http://www.w3.org/2004/02/skos/core#">
    <owl:Ontology rdf:about="http://vocab.linkeddata.es/datosabiertos/def/medio-ambiente/contaminacion-acustica">
        <dc:rights rdf:datatype="&xsd;string">Creative Commons Attribution 4.0 International (CC BY 4.0)</dc:rights>
        <ns:license rdf:datatype="&xsd;string">http://creativecommons.org/licenses/by/4.0/</ns:license>
        <dcterms:title xml:lang="en">Acoustic Pollution</dcterms:title>
        <dc:title xml:lang="en">Acoustic Pollution</dc:title>
        <dc:description xml:lang="en">The vocabulary extends W3C Semantic Sensor Network Ontology (SSN) with classes and properties to represent the data about acoustic pollution. Also it reuses OWL-Time Ontology to represent time and WGS84 Geo Positioning Ontology to represent spatial position through longitude, latitude and altitude.</dc:description>
        <dc:title xml:lang="es">Contaminación Acústica</dc:title>
        <dcterms:title xml:lang="es">Contaminación Acústica</dcterms:title>
        <dcterms:description xml:lang="es">Este vocabulario extiende la W3C Semantic Sensor Network Ontology (SSN) con clases y propiedades para representar los datos de la contaminación acústica. También se reutiliza la OWL Ontology of Time (OWL-Time)  para representar el tiempo y la WGS84 Geo Positioning Ontology para representar la posición en el espacio a través de la longitud, latitud y altitud</dcterms:description>
        <dc:description xml:lang="es">Este vocabulario extiende la W3C Semantic Sensor Network Ontology (SSN) con clases y propiedades para representar los datos de la contaminación acústica. También se reutiliza la OWL Ontology of Time (OWL-Time)  para representar el tiempo y la WGS84 Geo Positioning Ontology para representar la posición en el espacio a través de la longitud, latitud y altitud</dc:description>
        <dc:contributor xml:lang="es">Mariano Fernández López (Ontology Engineering Group)</dc:contributor>
        <dc:contributor xml:lang="es">María Poveda Villalón (Ontology Engineering Group)</dc:contributor>
        <dc:contributor xml:lang="es">Oscar Corcho García (Ontology Engineering Group)</dc:contributor>
        <dc:creator xml:lang="es">Paola Espinoza Arias (Ontology Engineering Group y Secretaría de Educación Superior, Ciencia, Tecnología e Innovación)</dc:creator>
        <dc:contributor xml:lang="es">Raúl García Castro (Ontology Engineering Group)</dc:contributor>
		<vann:preferredNamespaceUri rdf:resource="http://vocab.linkeddata.es/datosabiertos/def/medio-ambiente/contaminacion-acustica#"/>
		<vann:preferredNamespacePrefix>noise</vann:preferredNamespacePrefix>
        <owl:imports rdf:resource="http://purl.oclc.org/NET/ssnx/ssn"/>
        <owl:versionIRI rdf:resource="http://vocab.linkeddata.es/datosabiertos/def/medio-ambiente/contaminacion-acustica"/>
        <owl:imports rdf:resource="http://vocab.linkeddata.es/datosabiertos/kos/medio-ambiente/contaminacion-acustica"/>
        <owl:imports rdf:resource="http://www.w3.org/2006/time"/>
    </owl:Ontology>
    


    <!-- 
    ///////////////////////////////////////////////////////////////////////////////////////
    //
    // Annotation properties
    //
    ///////////////////////////////////////////////////////////////////////////////////////
     -->

    


    <!-- http://purl.org/dc/elements/1.1/contributor -->

    <owl:AnnotationProperty rdf:about="&dc;contributor"/>
    


    <!-- http://purl.org/dc/elements/1.1/description -->

    <owl:AnnotationProperty rdf:about="&dc;description"/>
    


    <!-- http://purl.org/vocab/vann/preferredNamespacePrefix -->

    <owl:AnnotationProperty rdf:about="&vann;preferredNamespacePrefix"/>
    


    <!-- http://purl.org/vocab/vann/preferredNamespaceUri -->

    <owl:AnnotationProperty rdf:about="&vann;preferredNamespaceUri"/>
    


    <!-- http://www.w3.org/1999/02/22-rdf-syntax-ns#value -->

    <owl:AnnotationProperty rdf:about="&rdf;value"/>
    


    <!-- http://www.w3.org/2003/01/geo/wgs84_pos#alt -->

    <owl:AnnotationProperty rdf:about="&wgs84_pos;alt">
        <rdfs:label rdf:datatype="&xsd;string">altitude</rdfs:label>
        <rdfs:comment rdf:datatype="&xsd;string">The WGS84 altitude of a SpatialThing (decimal meters 
above the local reference ellipsoid).</rdfs:comment>
        <rdfs:domain rdf:resource="&wgs84_pos;SpatialThing"/>
    </owl:AnnotationProperty>
    


    <!-- http://www.w3.org/2003/01/geo/wgs84_pos#lat -->

    <owl:AnnotationProperty rdf:about="&wgs84_pos;lat">
        <rdfs:label rdf:datatype="&xsd;string">latitude</rdfs:label>
        <rdfs:comment rdf:datatype="&xsd;string">The WGS84 latitude of a SpatialThing (decimal degrees).</rdfs:comment>
        <rdfs:domain rdf:resource="&wgs84_pos;SpatialThing"/>
    </owl:AnnotationProperty>
    


    <!-- http://www.w3.org/2003/01/geo/wgs84_pos#location -->

    <owl:AnnotationProperty rdf:about="&wgs84_pos;location">
        <rdfs:label rdf:datatype="&xsd;string">location</rdfs:label>
        <rdfs:comment rdf:datatype="&xsd;string">The relation between something and the point, 
 or other geometrical thing in space, where it is.  For example, the realtionship between
 a radio tower and a Point with a given lat and long.
 Or a relationship between a park and its outline as a closed arc of points, or a road and
 its location as a arc (a sequence of points).
 Clearly in practice there will be limit to the accuracy of any such statement, but one would expect
 an accuracy appropriate for the size of the object and uses such as mapping .
 </rdfs:comment>
        <rdfs:subPropertyOf rdf:resource="&foaf;based_near"/>
    </owl:AnnotationProperty>
    


    <!-- http://www.w3.org/2003/01/geo/wgs84_pos#long -->

    <owl:AnnotationProperty rdf:about="&wgs84_pos;long">
        <rdfs:label rdf:datatype="&xsd;string">longitude</rdfs:label>
        <rdfs:comment rdf:datatype="&xsd;string">The WGS84 longitude of a SpatialThing (decimal degrees).</rdfs:comment>
        <rdfs:domain rdf:resource="&wgs84_pos;SpatialThing"/>
    </owl:AnnotationProperty>
    


    <!-- http://xmlns.com/foaf/0.1/based_near -->

    <owl:AnnotationProperty rdf:about="&foaf;based_near"/>
    


    <!-- 
    ///////////////////////////////////////////////////////////////////////////////////////
    //
    // Object Properties
    //
    ///////////////////////////////////////////////////////////////////////////////////////
     -->

    


    <!-- http://purl.oclc.org/NET/ssnx/ssn#observationSamplingTime -->

    <rdf:Description rdf:about="http://purl.oclc.org/NET/ssnx/ssn#observationSamplingTime">
        <rdfs:domain rdf:resource="http://purl.oclc.org/NET/ssnx/ssn#ObservationValue"/>
        <rdfs:range rdf:resource="http://www.w3.org/2006/time#TemporalEntity"/>
    </rdf:Description>
    


    <!-- http://vocab.linkeddata.es/datosabiertos/def/medio-ambiente/contaminacion-acustica#belongsToSensorClass -->

    <owl:ObjectProperty rdf:about="&noise;belongsToSensorClass">
        <rdfs:label xml:lang="en">belongs to sensor class</rdfs:label>
        <rdfs:label xml:lang="es">pertenece a una clase de sensor</rdfs:label>
        <rdfs:comment xml:lang="en">Noise sensor may or may not belong to a class. The class defines the technical characteristics of the sensor that establish the limits of acceptance and the range of operating temperatures.</rdfs:comment>
        <rdfs:comment xml:lang="es">El sensor de ruido puede pertenecer o no a una clase. La clase define las caracterísiticas técnicas del sensor que establecen los límites de aceptación y el rango de temperaturas de funcionamiento.</rdfs:comment>
        <rdfs:domain rdf:resource="&noise;NoiseSensor"/>
        <rdfs:range rdf:resource="&skos;Concept"/>
    </owl:ObjectProperty>
    


    <!-- http://vocab.linkeddata.es/datosabiertos/def/medio-ambiente/contaminacion-acustica#hasAcousticEmitter -->

    <owl:ObjectProperty rdf:about="&noise;hasAcousticEmitter">
        <rdfs:label xml:lang="en">has acoustic emitter</rdfs:label>
        <rdfs:label xml:lang="es">tiene emisor acústico</rdfs:label>
        <rdfs:comment xml:lang="en">Noise level is caused by an acoustic emitter.</rdfs:comment>
        <rdfs:comment xml:lang="es">El nivel de ruido tiene un emisor acústico que lo provoca.</rdfs:comment>
        <rdfs:domain rdf:resource="&noise;NoiseLevel"/>
        <rdfs:range rdf:resource="&skos;Concept"/>
    </owl:ObjectProperty>
    


    <!-- http://vocab.linkeddata.es/datosabiertos/def/medio-ambiente/contaminacion-acustica#hasUnitOfMeasure -->

    <owl:ObjectProperty rdf:about="&noise;hasUnitOfMeasure">
        <rdfs:label xml:lang="en">has unit of measure</rdfs:label>
        <rdfs:label xml:lang="es">tiene unidad de medida</rdfs:label>
        <rdfs:comment xml:lang="en">Relationship between the measured value by the sensor and the unit of measure of this value.</rdfs:comment>
        <rdfs:comment xml:lang="es">Relación entre el valor medido por el sensor y  la unidad de medida en la que este valor es expresado.</rdfs:comment>
        <rdfs:domain rdf:resource="http://purl.oclc.org/NET/ssnx/ssn#SensorOutput"/>
        <rdfs:range rdf:resource="http://www.wurvoc.org/vocabularies/om-1.8/Unit_of_measure"/>
    </owl:ObjectProperty>
    


    <!-- http://vocab.linkeddata.es/datosabiertos/def/medio-ambiente/contaminacion-acustica#isWeightingWith -->

    <owl:ObjectProperty rdf:about="&noise;isWeightingWith">
        <rdfs:label xml:lang="en">is weighting with</rdfs:label>
        <rdfs:label xml:lang="es">es ponderado con</rdfs:label>
        <rdfs:comment xml:lang="en">The measurement performed by the Noise Sensor has a frequency weighting. It can be without weighting (Z), weighting A or C.</rdfs:comment>
        <rdfs:comment xml:lang="es">La medida que realiza el Sensor de Ruido tiene una ponderación frecuencial. Puede ser sin poderación (Z), ponderación A o C.</rdfs:comment>
        <rdfs:domain rdf:resource="http://purl.oclc.org/NET/ssnx/ssn#ObservationValue"/>
        <rdfs:range rdf:resource="&noise;Weighting"/>
    </owl:ObjectProperty>
    


    <!-- http://vocab.linkeddata.es/datosabiertos/def/medio-ambiente/contaminacion-acustica#lastCalibrationDate -->

    <owl:ObjectProperty rdf:about="&noise;lastCalibrationDate">
        <rdfs:label xml:lang="en">last calibration date</rdfs:label>
        <rdfs:label xml:lang="es">última fecha de calibración del sensor.</rdfs:label>
        <rdfs:comment xml:lang="en">Last calibration date of the sensor. Calibration is a periodic process performed on acoustic sensors to verify their correct operation in their different working modes.</rdfs:comment>
        <rdfs:comment xml:lang="es">Última fecha de calibración del sensor.  La calibración es un proceso periódico realizado a los sensores acústicos para verificar su correcto funcionamiento en sus distintos modos de trabajo.</rdfs:comment>
        <rdfs:domain rdf:resource="&noise;NoiseSensor"/>
        <rdfs:range rdf:resource="http://www.w3.org/2006/time#Instant"/>
    </owl:ObjectProperty>
    


    <!-- http://vocab.linkeddata.es/datosabiertos/def/medio-ambiente/contaminacion-acustica#referenceInterval -->

    <owl:ObjectProperty rdf:about="&noise;referenceInterval">
        <rdfs:label xml:lang="en">reference interval</rdfs:label>
        <rdfs:label xml:lang="es">intervalo de referencia</rdfs:label>
        <rdfs:comment xml:lang="en">Interval of time where the noise assessment was performed. The reference time interval can be specified in national or international standards or by local authorities to encompass typical human activities and variations in the operation of noise sources. The reference time intervals can be for example: a part of the day, a whole day or a complete week. Some countries may even define longer reference intervals.</rdfs:comment>
        <rdfs:seeAlso xml:lang="es">ISO 1996-1: 2005</rdfs:seeAlso>
        <rdfs:comment xml:lang="es">Intervalo de tiempo al que se refiere la evaluación del ruido. El intervalo de tiempo de referencia se puede especificar en normas nacionales o internacionales o por las autoridades locales para englobar las actividades humanas típicas y las variaciones en el funcionamiento de las fuentes de ruido. Los intervalos de tiempo de referencia pueden ser por ejemplo: una parte del día, un día entero o una semana completa. Algunos países pueden definir incluso intervalos de referencia más largos.</rdfs:comment>
        <rdfs:domain rdf:resource="&noise;NoiseLevel"/>
        <rdfs:range rdf:resource="http://www.w3.org/2006/time#TemporalEntity"/>
    </owl:ObjectProperty>
    


    <!-- http://www.w3.org/2003/01/geo/wgs84_pos#location -->

    <owl:ObjectProperty rdf:about="&wgs84_pos;location">
        <rdfs:label rdf:datatype="&xsd;string">location</rdfs:label>
        <rdfs:comment rdf:datatype="&xsd;string">The relation between something and the point, 
 or other geometrical thing in space, where it is.  For example, the realtionship between
 a radio tower and a Point with a given lat and long.
 Or a relationship between a park and its outline as a closed arc of points, or a road and
 its location as a arc (a sequence of points).
 Clearly in practice there will be limit to the accuracy of any such statement, but one would expect
 an accuracy appropriate for the size of the object and uses such as mapping .
 </rdfs:comment>
        <rdfs:range rdf:resource="&wgs84_pos;SpatialThing"/>
    </owl:ObjectProperty>
    


    <!-- 
    ///////////////////////////////////////////////////////////////////////////////////////
    //
    // Data properties
    //
    ///////////////////////////////////////////////////////////////////////////////////////
     -->

    


    <!-- http://www.co-ode.org/ontologies/ont.owl#timePercentage -->

    <owl:DatatypeProperty rdf:about="http://www.co-ode.org/ontologies/ont.owl#timePercentage">
        <rdfs:label xml:lang="en">Time percentage</rdfs:label>
        <rdfs:label xml:lang="es">Porcentaje de tiempo</rdfs:label>
        <rdfs:comment xml:lang="en">Percentage of time (N%) of the reference time interval where the noise level is exceeded.</rdfs:comment>
        <rdfs:comment xml:lang="es">Porcentaje de tiempo (N%) del intervalo de tiempo de referencia en el que se excede el nivel de ruido.</rdfs:comment>
        <rdfs:domain rdf:resource="&noise;PercentilNoiseLevel"/>
        <rdfs:range rdf:resource="&xsd;double"/>
    </owl:DatatypeProperty>
    


    <!-- 
    ///////////////////////////////////////////////////////////////////////////////////////
    //
    // Classes
    //
    ///////////////////////////////////////////////////////////////////////////////////////
     -->

    


    <!-- http://vocab.linkeddata.es/datosabiertos/def/medio-ambiente/contaminacion-acustica#AverageNoiseLevel -->

    <owl:Class rdf:about="&noise;AverageNoiseLevel">
        <rdfs:label xml:lang="en">Average Noise Level</rdfs:label>
        <rdfs:label xml:lang="es">Nivel Medio de Ruido</rdfs:label>
        <rdfs:subClassOf rdf:resource="&noise;NoiseLevel"/>
        <rdfs:comment xml:lang="en">Average sound pressure level that has been measured by the sensor.</rdfs:comment>
        <rdfs:comment xml:lang="es">Nivel medio de presión sonora que ha sido medido por el sensor.</rdfs:comment>
    </owl:Class>
    


    <!-- http://vocab.linkeddata.es/datosabiertos/def/medio-ambiente/contaminacion-acustica#NoiseLevel -->

    <owl:Class rdf:about="&noise;NoiseLevel">
        <rdfs:label xml:lang="en">Noise Level</rdfs:label>
        <rdfs:label xml:lang="es">Nivel de Ruido</rdfs:label>
        <rdfs:subClassOf rdf:resource="http://purl.oclc.org/NET/ssnx/ssn#Property"/>
        <rdfs:comment xml:lang="en">Sound pressure level measured by the sensor. It is a physical magnitude describing acoustic pollution and related to the produced effects. It is measured in decibels (dB).</rdfs:comment>
        <rdfs:comment xml:lang="es">Nivel de presión sonora que ha sido medido por el sensor. Es una magnitud física para describir la contaminación acústica, que tiene relación con los efectos producidos por ésta. Se mide en decibelios (dB).</rdfs:comment>
    </owl:Class>
    


    <!-- http://vocab.linkeddata.es/datosabiertos/def/medio-ambiente/contaminacion-acustica#NoiseSensor -->

    <owl:Class rdf:about="&noise;NoiseSensor">
        <rdfs:label xml:lang="en">Noise Sensor</rdfs:label>
        <rdfs:label xml:lang="es">Sensor de Ruido</rdfs:label>
        <rdfs:subClassOf rdf:resource="http://purl.oclc.org/NET/ssnx/ssn#SensingDevice"/>
        <rdfs:comment xml:lang="en">Device that measures the noise level. It detects changes in the air pressure, at a certain location and at a given time, and converts them into electrical pulses. These electric pulses have a frequency, representing the acoustic waves. The frequency range perceived human beings is from 20 Hz to 20 kHz.</rdfs:comment>
        <rdfs:comment xml:lang="es">Dispositivo que mide el nivel de ruido. Detecta los cambios en la presión del aire, en determinado lugar y en un momento dado, y los  convierte en pulso eléctricos. Estos pulsos eléctricos tienen una frecuencia, que es la de las ondas acústicas. El rango de frecuencia que percibe el ser humano es de 20 Hz a 20 kHz.</rdfs:comment>
    </owl:Class>
    


    <!-- http://vocab.linkeddata.es/datosabiertos/def/medio-ambiente/contaminacion-acustica#PercentilNoiseLevel -->

    <owl:Class rdf:about="&noise;PercentilNoiseLevel">
        <rdfs:label xml:lang="en">Percentil Noise Level</rdfs:label>
        <rdfs:label xml:lang="es">Nivel de Ruido en Percentiles</rdfs:label>
        <rdfs:subClassOf rdf:resource="&noise;NoiseLevel"/>
        <rdfs:comment xml:lang="en">Weighted frequency and time sound pressure level exceeding the N% of time of the considered interval.</rdfs:comment>
        <rdfs:seeAlso xml:lang="es">AENOR: UNE-ISO 1996-1</rdfs:seeAlso>
        <rdfs:comment xml:lang="es">Nivel de presión sonora ponderado en frecuencia y ponderado en el tiempo superado el N% de tiempo del intervalo considerado.</rdfs:comment>
    </owl:Class>
    


    <!-- http://vocab.linkeddata.es/datosabiertos/def/medio-ambiente/contaminacion-acustica#Weighting -->

    <owl:Class rdf:about="&noise;Weighting">
        <rdfs:label xml:lang="en">Weighting</rdfs:label>
        <rdfs:label xml:lang="es">Ponderación</rdfs:label>
        <rdfs:subClassOf rdf:resource="http://www.loa-cnr.it/ontologies/DUL.owl#Method"/>
        <rdfs:comment xml:lang="en">The measurement performed by the Noise Sensor has a frequency weighting that is used for a correct interpretation and measurement of the loudness levels of a particular sound compared to the non-linear nature of the human ear for the different frequencies of the audible spectrum. It can be without weighting (Z), weighting A or C.</rdfs:comment>
        <rdfs:comment xml:lang="es">La medida que realiza el Sensor de Ruido tiene una ponderación frecuencial que se utiliza para una correcta interpretación y medición de  los  niveles  de  sonoridad  de  un  determinado  sonido  en  comparación  con  la naturaleza  no  lineal  del  oído  humano  para  las  distintas  frecuencias  del  espectro audible. Puede ser sin poderación (Z), ponderación A o C.</rdfs:comment>
    </owl:Class>
    


    <!-- http://www.w3.org/2003/01/geo/wgs84_pos#Point -->

    <owl:Class rdf:about="&wgs84_pos;Point">
        <rdfs:label rdf:datatype="&xsd;string">point</rdfs:label>
        <rdfs:subClassOf rdf:resource="&wgs84_pos;SpatialThing"/>
        <rdfs:comment rdf:datatype="&xsd;string"> 
Uniquely identified by lat/long/alt. i.e.

spaciallyIntersects(P1, P2) :- lat(P1, LAT), long(P1, LONG), alt(P1, ALT),
  lat(P2, LAT), long(P2, LONG), alt(P2, ALT).

sameThing(P1, P2) :- type(P1, Point), type(P2, Point), spaciallyIntersects(P1, P2).
  </rdfs:comment>
        <rdfs:comment rdf:datatype="&xsd;string">A point, typically described using a coordinate system relative to Earth, such as WGS84.
  </rdfs:comment>
    </owl:Class>
    


    <!-- http://www.w3.org/2003/01/geo/wgs84_pos#SpatialThing -->

    <owl:Class rdf:about="&wgs84_pos;SpatialThing">
        <rdfs:label rdf:datatype="&xsd;string">SpatialThing</rdfs:label>
        <rdfs:comment rdf:datatype="&xsd;string">Anything with spatial extent, i.e. size, shape, or position.
 e.g. people, places, bowling balls, as well as abstract areas like cubes.
</rdfs:comment>
    </owl:Class>
    


    <!-- http://www.w3.org/2004/02/skos/core#Concept -->

    <owl:Class rdf:about="&skos;Concept"/>
    


    <!-- http://www.wurvoc.org/vocabularies/om-1.8/Unit_of_measure -->

    <owl:Class rdf:about="http://www.wurvoc.org/vocabularies/om-1.8/Unit_of_measure">
        <rdfs:label xml:lang="en">Unit of Measure</rdfs:label>
        <rdfs:label xml:lang="es">Unidad de Medida</rdfs:label>
        <rdfs:isDefinedBy rdf:datatype="&xsd;string">http://www.wurvoc.org/vocabularies/om-1.8/</rdfs:isDefinedBy>
        <rdfs:comment xml:lang="en">A unit of measure is a definite magnitude of a quantity, defined and adopted by convention and/or by law. It is used as a standard for measurement of the same quantity, where any other value of the quantity can be expressed as a simple multiple of the unit of measure. For example, length is a quantity; the metre is a unit of length that represents a definite predetermined length. When we say 10 metre (or 10 m), we actually mean 10 times the definite predetermined length called &quot;metre&quot;.</rdfs:comment>
        <rdfs:comment xml:lang="es">Una unidad de medida es una magnitud definida de una cantidad, definida y adoptada por convención y / o por ley. Se utiliza como estándar para medir la misma cantidad, donde cualquier otro valor de la cantidad puede expresarse como un simple múltiplo de la unidad de medida. Por ejemplo, longitud es una cantidad; El metro es una unidad de longitud que representa una longitud predeterminada definida. Cuando decimos 10 metros (o 10 m), en realidad decimos 10 veces la longitud predeterminada definida llamada &quot;metro&quot;. (definición tomada de la ontología om).</rdfs:comment>
    </owl:Class>
    


    <!-- 
    ///////////////////////////////////////////////////////////////////////////////////////
    //
    // Individuals
    //
    ///////////////////////////////////////////////////////////////////////////////////////
     -->

    


    <!-- http://dbpedia.org/resource/Decibel -->

    <owl:NamedIndividual rdf:about="http://dbpedia.org/resource/Decibel">
        <rdf:type rdf:resource="http://www.wurvoc.org/vocabularies/om-1.8/Unit_of_measure"/>
    </owl:NamedIndividual>
    


    <!-- http://vocab.linkeddata.es/datosabiertos/def/medio-ambiente/contaminacion-acustica#ClaseI -->

    <owl:NamedIndividual rdf:about="&noise;ClaseI">
        <rdf:type rdf:resource="&skos;Concept"/>
        <rdfs:label xml:lang="en">Class I</rdfs:label>
        <rdfs:label xml:lang="es">Clase I</rdfs:label>
        <rdfs:comment xml:lang="en">Sensor that fulfills the most restrictive precision characteristics defined in the IEC standard. This class of sensors has smaller tolerance margins in its measurement range. Class I instruments are specified within the air temperature range from -10 ° C to +50 ° C.</rdfs:comment>
        <rdfs:seeAlso xml:lang="es">Norma IEC 61672-1:2013</rdfs:seeAlso>
        <rdfs:comment xml:lang="es">Sensor que cumple las características de precisión más restrictivas definidas en la normativa IEC. Esta clase de sensores tiene menores márgenes de tolerancia en su rango de medida. Los instrumentos de Clase I se especifican dentro del rango de temperaturas del aire desde -10 ºC  hasta  +50 ºC.</rdfs:comment>
    </owl:NamedIndividual>
    


    <!-- http://vocab.linkeddata.es/datosabiertos/def/medio-ambiente/contaminacion-acustica#ClaseII -->

    <owl:NamedIndividual rdf:about="&noise;ClaseII">
        <rdf:type rdf:resource="&skos;Concept"/>
        <rdfs:label xml:lang="en">Class II</rdfs:label>
        <rdfs:label xml:lang="es">Clase II</rdfs:label>
        <rdfs:comment xml:lang="en">Sensor that fulfills the less restrictive precision characteristics defined in the IEC standard. This class of sensors has greater tolerance margins in its measuring range. Class II instruments are specified within the air temperature range from 0 ° C to + 40 ° C.</rdfs:comment>
        <rdfs:seeAlso xml:lang="es">Norma IEC 61672-1:2013</rdfs:seeAlso>
        <rdfs:comment xml:lang="es">Sensor que cumple las características de precisión menos restrictivas definidas en la normativa IEC. Esta clase de sensores tiene mayores márgenes de tolerancia en su rango de medida. Los instrumentos de Clase II se especifican dentro del rango de temperaturas del aire desde 0 ºC  hasta  +40 ºC.</rdfs:comment>
    </owl:NamedIndividual>
    


    <!-- http://vocab.linkeddata.es/datosabiertos/def/medio-ambiente/contaminacion-acustica#PonderacionA -->

    <owl:NamedIndividual rdf:about="&noise;PonderacionA">
        <rdf:type rdf:resource="&noise;Weighting"/>
        <rdf:type rdf:resource="&skos;Concept"/>
        <rdfs:label xml:lang="en">Weighting A</rdfs:label>
        <rdfs:label xml:lang="es">Ponderación A</rdfs:label>
        <rdfs:comment xml:lang="en">More common weighting in enviromental acoustic. It is used to adjust noise levels as the human ear perceives them.</rdfs:comment>
        <rdfs:seeAlso xml:lang="es">Norma IEC 61672:2003</rdfs:seeAlso>
        <rdfs:comment xml:lang="es">Ponderación más habitual en acústica ambiental. Se utiliza para ajustar los niveles de ruido a cómo los percibe el oido humano.</rdfs:comment>
    </owl:NamedIndividual>
    


    <!-- http://vocab.linkeddata.es/datosabiertos/def/medio-ambiente/contaminacion-acustica#PonderacionC -->

    <owl:NamedIndividual rdf:about="&noise;PonderacionC">
        <rdf:type rdf:resource="&noise;Weighting"/>
        <rdf:type rdf:resource="&skos;Concept"/>
        <rdfs:label xml:lang="en">Weighting C</rdfs:label>
        <rdfs:label xml:lang="es">Ponderación C</rdfs:label>
        <rdfs:comment xml:lang="en">Weighting used to evaluate high noise leves.</rdfs:comment>
        <rdfs:seeAlso xml:lang="es">Norma IEC 61672:2003</rdfs:seeAlso>
        <rdfs:comment xml:lang="es">Ponderación que se utiliza para evaluar altos niveles de ruido.</rdfs:comment>
    </owl:NamedIndividual>
    


    <!-- http://vocab.linkeddata.es/datosabiertos/def/medio-ambiente/contaminacion-acustica#PonderacionZ -->

    <owl:NamedIndividual rdf:about="&noise;PonderacionZ">
        <rdf:type rdf:resource="&noise;Weighting"/>
        <rdf:type rdf:resource="&skos;Concept"/>
        <rdfs:label xml:lang="en">Weighting Z</rdfs:label>
        <rdfs:label xml:lang="es">Ponderación Z</rdfs:label>
        <rdfs:comment xml:lang="en">It represents the fact of not applying any type of frequency weighting to the sound waves captured by the noise sensor. They are captured as they are.</rdfs:comment>
        <rdfs:seeAlso xml:lang="es">Norma IEC 61672:2003</rdfs:seeAlso>
        <rdfs:comment xml:lang="es">Representa el hecho de no aplicar ningún tipo de ponderación frecuencial a las ondas sonoras captadas por el sensor de ruido. Se captan tal y como son.</rdfs:comment>
    </owl:NamedIndividual>
    


    <!-- 
    ///////////////////////////////////////////////////////////////////////////////////////
    //
    // Annotations
    //
    ///////////////////////////////////////////////////////////////////////////////////////
     -->

    <rdf:Description rdf:about="&wgs84_pos;lat_long">
        <rdfs:label rdf:datatype="&xsd;string">lat/long</rdfs:label>
        <rdfs:comment rdf:datatype="&xsd;string">A comma-separated representation of a latitude, longitude coordinate.</rdfs:comment>
    </rdf:Description>
    <rdf:Description rdf:about="http://www.w3.org/2003/01/geo/wgs84_pos#">
        <rdfs:label rdf:datatype="&xsd;string">geo</rdfs:label>
        <rdfs:comment rdf:datatype="&xsd;string">
Recent changes to this namespace:
$Log: wgs84_pos.rdf,v $
Revision 1.22  2009/04/20 15:00:30  timbl
Remove the time bits which have been deal with elsewhere eg in iCal.

Revision 1.21  2009/04/20 12:52:47  timbl
try again

Revision 1.20  2009/04/20 12:42:11  timbl
Add Event (edited ages ago and never checked in), and location (following discussion http://chatlogs.planetrdf.com/swig/2009-04-20#T12-36-09)

Revision 1.19  2009/04/20 12:36:31  timbl
Add Event (edited ages ago and never checked in), and location (following discussion http://chatlogs.planetrdf.com/swig/2009-04-20#T12-36-09)

Revision 1.18  2006/02/01 22:01:04  danbri
Clarified that lat and long are decimal degrees, and that alt is decimal metres about local reference ellipsoid

Revision 1.17  2004/02/06 17:38:12  danbri
Fixed a bad commit screwup

Revision 1.15  2003/04/19 11:24:08  danbri
Fixed the typo even more.

Revision 1.14  2003/04/19 11:16:56  danbri
fixed a typo

Revision 1.13  2003/02/19 22:27:27  connolly
relaxed domain constraints on lat/long/alt from Point to SpatialThing

Revision 1.12  2003/01/12 01:41:41  danbri
Trying local copy of XSLT doc.

Revision 1.11  2003/01/12 01:20:18  danbri
added a link to morten&apos;s xslt rdfs viewer.

Revision 1.10  2003/01/11 18:56:49  danbri
Removed datatype range from lat and long properties, since they would
have required each occurance of the property to mention the datatype.

Revision 1.9  2003/01/11 11:41:31  danbri
Another typo; repaired rdfs:Property to rdf:Property x4

Revision 1.8  2003/01/11 11:05:02  danbri
Added an rdfs:range for each lat/long/alt property,
http://www.w3.org/2001/XMLSchema#float

Revision 1.7  2003/01/10 20:25:16  danbri
Longer rdfs:comment for Point, trying to be Earth-centric and neutral about
coordinate system(s) at the same time. Feedback welcomed.

Revision 1.6  2003/01/10 20:18:30  danbri
Added CVS log comments into the RDF/XML as an rdfs:comment property of the
vocabulary. Note that this is not common practice (but seems both harmless
and potentially useful).


revision 1.5
date: 2003/01/10 20:14:31;  author: danbri;  state: Exp;  lines: +16 -5
Updated schema:
Added a dc:date, added url for more info. Changed the rdfs:label of the
namespace from gp to geo. Added a class Point, set as the rdfs:domain of
each property. Added XML comment on the lat_long property suggesting that
we might not need it (based on #rdfig commentary from implementors).

revision 1.4
date: 2003/01/10 20:01:07;  author: danbri;  state: Exp;  lines: +6 -5
Fixed typo; several rdfs:about attributes are now rdf:about. Thanks to MortenF in
#rdfig for catching this error.

revision 1.3
date: 2003/01/10 11:59:03;  author: danbri;  state: Exp;  lines: +4 -3
fixed buglet in vocab, added more wgs links

revision 1.2
date: 2003/01/10 11:01:11;  author: danbri;  state: Exp;  lines: +4 -4
Removed alt from the as-a-flat-string property, and switched from
space separated to comma separated.

revision 1.1
date: 2003/01/10 10:53:23;  author: danbri;  state: Exp;
basic geo vocab

</rdfs:comment>
        <dc:date rdf:datatype="&xsd;string">$Date: 2009/04/20 15:00:30 $</dc:date>
        <dc:description rdf:datatype="&xsd;string">A vocabulary for representing latitude, longitude and 
 altitude information in the WGS84 geodetic reference datum. 
 Version $Id: wgs84_pos.rdf,v 1.22 2009/04/20 15:00:30 timbl Exp $. See http://www.w3.org/2003/01/geo/ for more details.</dc:description>
        <dc:title rdf:datatype="&xsd;string">WGS84 Geo Positioning: an RDF vocabulary</dc:title>
    </rdf:Description>
</rdf:RDF>



<!-- Generated by the OWL API (version 3.4.2) http://owlapi.sourceforge.net -->

